Make progress on the proofs of VarsOfExpr

src/Transforms/VarsOfExpr.dfy
@@ -23,17 +23,17 @@ module Bootstrap.Transforms.VarsOfExpr {
   import opened Generic
   import Shallow
 
-  type Environment = Interp.Environment
-  type State = Interp.State
-  type Expr = Interp.Expr
+  type {:verify false} Environment = Interp.Environment
+  type {:verify false} State = Interp.State
+  type {:verify false} Expr = Interp.Expr
 
-  function method {:opaque} SeqToSet<T>(s: seq<T>): set<T>
+  function method {:verify false} {:opaque} SeqToSet<T>(s: seq<T>): set<T>
     // Unfortunately, we need this small opaque helper to prevent with proof explosions.
   {
     set x | x in s
   }
 
-  function method {:opaque} VarsToNameSet(vars: seq<Exprs.TypedVar>): set<string>
+  function method {:verify false} {:opaque} VarsToNameSet(vars: seq<Exprs.TypedVar>): set<string>
     // Same as for ``SeqToSet``: making this definition opaque is annoying, but we need it to
     // prevent proof explosions.
   {
@@ -41,7 +41,7 @@ module Bootstrap.Transforms.VarsOfExpr {
   }
 
   // TODO(SMH): move?
-  function method VarsOfExpr(read: bool, e: Syntax.Expr): set<string>
+  function method {:verify false} VarsOfExpr(read: bool, e: Syntax.Expr): set<string>
     decreases e.Size(), 0
     // Return the set of all variables used in an expression (accessed, updated or even declared).
     //
@@ -69,29 +69,29 @@ module Bootstrap.Transforms.VarsOfExpr {
     }
   }
 
-  function method VarsOfExprs(read: bool, es: seq<Syntax.Expr>): set<string>
+  function method {:verify false} VarsOfExprs(read: bool, es: seq<Syntax.Expr>): set<string>
     decreases Expr.Exprs_Size(es), 1
   {
     if es == [] then {}
     else VarsOfExpr(read, es[0]) + VarsOfExprs(read, es[1..])
   }
 
-  function method UpdtVarsOfExpr(e: Syntax.Expr): set<string>
+  function method {:verify false} UpdtVarsOfExpr(e: Syntax.Expr): set<string>
   {
     VarsOfExpr(false, e)
   }
 
-  function method UpdtVarsOfExprs(es: seq<Syntax.Expr>): set<string>
+  function method {:verify false} UpdtVarsOfExprs(es: seq<Syntax.Expr>): set<string>
   {
     VarsOfExprs(false, es)
   }
 
-  function method AllVarsOfExpr(e: Syntax.Expr): set<string>
+  function method {:verify false} AllVarsOfExpr(e: Syntax.Expr): set<string>
   {
     VarsOfExpr(true, e)
   }
 
-  function method AllVarsOfExprs(es: seq<Syntax.Expr>): set<string>
+  function method {:verify false} AllVarsOfExprs(es: seq<Syntax.Expr>): set<string>
   {
     VarsOfExprs(true, es)
   }
@@ -99,16 +99,17 @@ module Bootstrap.Transforms.VarsOfExpr {
   // Accumulator used for substitutions.
   // `subst`: the substitution
   // `frozen`: the variables which appear in the expressions with which we substitute
-  datatype SubstAcc = SubstAcc(subst: map<string, Expr>)//, frozen: set<string>)
+  datatype {:verify false} SubstAcc = SubstAcc(subst: map<string, Expr>)//, frozen: set<string>)
 
-  predicate method NotVarDecl(e: Syntax.Expr)
+  predicate method {:verify false} NotVarDecl(e: Syntax.Expr)
   {
     !e.VarDecl?
   }
 }
 
 // Rem.(SMH): about the name, see the comment for `Bootstrap.Transforms.VarsOfExpr`
-module Bootstrap.Transforms.VarsOfExprUselessBindings.Base {
+module Bootstrap.Transforms.VarsOfExprAddUselessBindings refines Semantics.ExprInduction {
+  // TODO(SMH): update this comment
   // This module proves that:
   // If:
   // - we have an expression `e` and contexts `ctx` and `ctx'`
@@ -116,5 +117,650 @@ module Bootstrap.Transforms.VarsOfExprUselessBindings.Base {
   // Then:
   // - evaluating `e` starting from `ctx` and `ctx'` leads to similar results
 
+  import opened Semantics.Pure
+//  import opened Base
+  import opened VarsOfExpr
+//  import Semantics.InterpStateIneq
+//  import Semantics.EqInterpRefl
+
+  type {:verify false} Value = Interp.Value
+
+  type {:verify false} Context = Interp.Context
+
+  const {:verify false} EmptyCtx: Context := map[]
+
+  datatype {:verify false} MState = MState(env: Environment, add: map<string, Value>, ctx: State)
+  datatype MValue = MValue(v: Value, v': Value)
+  datatype MSeqValue = MSeqValue(vs: seq<Value>, vs': seq<Value>)
+
+/*  predicate EqOuterRollback(outer_rollback: Context, ctx: State, outer_rollback': Context, ctx': State)
+  {
+    EqCtx(ctx.rollback + outer_rollback, ctx'.rollback + outer_rollback')
+  }*/
+
+/*  // TODO(SMH): move?
+  predicate {:verify false} {:opaque} EqSubCtx(keys: set<string>, ctx: Context, ctx': Context)
+  {
+    && keys <= ctx.Keys
+    && keys <= ctx'.Keys
+    // Rem.(SMH): we use a strong equality
+    && forall x | x in keys :: ctx[x] == ctx'[x] // EqValue(ctx[x], ctx'[x])
+  }*/
+
+/*  // TODO(SMH): move? This is not used in this module. But this should be kept with ``EqOuterRollback``
+  predicate {:verify false} EqRolled(keys: set<string>, ctx: State, ctx': State)
+  {
+    EqSubCtx(keys, ctx.locals + ctx.rollback, ctx'.locals + ctx'.rollback)
+  }*/
+
+//  predicate EqOnAdd(add: map<string, Value>, ctx: State, ctx': State)
+
+  predicate {:verify false} {:opaque} EqStateWithAdd(add: map<string, Value>, ctx: State, ctx': State)
+  {
+    //    && ctx.locals.Keys !! add.Keys
+    && EqCtx(ctx.locals, ctx'.locals - add.Keys)
+    && add.Keys <= ctx'.locals.Keys
+    && forall x | x in add.Keys :: ctx'.locals[x] == add[x]
+    && ctx.rollback == ctx'.rollback == map []
+  }
+
+/*  predicate EqResult<V>(eq_value: (V,V) -> bool, core: set<string>, res: InterpResult<V>, res': InterpResult<V>)
+  {
+    match (res, res')
+      case (Success(Return(v, ctx)), Success(Return(v', ctx'))) =>
+        && eq_value(v, v')
+        && EqStateWithCore(core, ctx, ctx')
+      case (Failure(_), _) => true
+      case _ => false
+  }
+
+  predicate {:verify false} EqResultValue(outer_rollback: Context, res: InterpResult<Value>, outer_rollback': Context, res': InterpResult<Value>)
+  {
+    EqResult(EqValue, outer_rollback, res, outer_rollback', res')
+  }
+
+  predicate {:verify false} EqResultSeqValue(outer_rollback: Context, res: InterpResult<seq<Value>>, outer_rollback': Context, res': InterpResult<seq<Value>>)
+  {
+    EqResult(EqSeqValue, outer_rollback, res, outer_rollback', res')
+  }
+
+  // TODO(SMH): factorize with EqResult and move. The annoying thing is that functions are not curried, so it makes
+  // facorization a bit hard...
+  predicate {:verify false} EqResultRolled<V>(eq_value: (V,V) -> bool, keys: set<string>, res: InterpResult<V>, res': InterpResult<V>)
+  {
+    match (res, res')
+      case (Success(Return(v, ctx)), Success(Return(v', ctx'))) =>
+        && eq_value(v, v')
+        && EqRolled(keys, ctx, ctx')
+      case (Failure(_), _) => true
+      case _ => false
+  }
+
+  predicate {:verify false} EqResultRolledValue(keys: set<string>, res: InterpResult<Value>, res': InterpResult<Value>)
+  {
+    EqResultRolled(EqValue, keys, res, res')
+  }
+
+  predicate {:verify false} EqResultRolledSeqValue(keys: set<string>, res: InterpResult<seq<Value>>, res': InterpResult<seq<Value>>)
+  {
+    EqResultRolled(EqSeqValue, keys, res, res')
+  }*/
+
+  predicate {:verify false} {:opaque} Inv(st: MState)
+  {
+    && st.ctx.locals.Keys !! st.add.Keys
+    && st.ctx.rollback == map []
+    //&& EqStateWithAdd(st.add, st.ctx)
+  }
+
+  predicate {:verify false} {:opaque} ExprValid(st: S, e: Expr)
+  {
+    && Deep.All_Expr(e, NotVarDecl)
+    // We don't need to use the Deep predicate (it is actually equivalent to not using it) but
+    // that makes the proofs easier.
+    // TODO(SMH): prove the corresponding lemma
+    && Deep.All_Expr(
+      e, var f := (e: Syntax.Expr) => st.add.Keys !! AllVarsOfExpr(e); f)
+  }
+
+  predicate {:verify false} ExprsValid(st: S, es: seq<Expr>)
+  {
+    forall e | e in es :: ExprValid(st, e)
+  }
+
+  type {:verify false} S(!new) = MState
+  type {:verify false} V(!new) = MValue
+  type {:verify false} VS(!new) = vs:MSeqValue | |vs.vs| == |vs.vs'| witness MSeqValue([], [])
+
+  predicate {:verify false} P(st: S, e: Expr)
+  {
+    var ctx := st.ctx;
+    var ctx' := ctx.(locals := ctx.locals + st.add);
+    var res := InterpExpr(e, st.env, ctx);
+    var res' := InterpExpr(e, st.env, ctx');
+    Inv(st) ==>
+    ExprValid(st, e) ==>
+    && (match (res, res') {
+        case (Success(Return(v1, ctx1)), Success(Return(v1', ctx1'))) =>
+          var st1 := MState(st.env, st.add, ctx1);
+          && EqValue(v1, v1')
+          && Inv(st1)
+          && EqStateWithAdd(st.add, ctx1, ctx1')
+        case (Failure(_), _) => true
+        case _ => false
+      })
+  }
   
+  predicate {:verify false} P_Succ(st: S, e: Expr, st': S, v: V)
+  {
+    var ctx := st.ctx;
+    var ctx' := ctx.(locals := ctx.locals + st.add);
+    var res := InterpExpr(e, st.env, ctx);
+    var res' := InterpExpr(e, st.env, ctx');
+    && Inv(st)
+    && ExprValid(st, e)
+    && (match (res, res') {
+        case (Success(Return(v1, ctx1)), Success(Return(v1', ctx1'))) =>
+          var st1 := MState(st.env, st.add, ctx1);
+          && EqValue(v1, v1')
+          && Inv(st1)
+          && EqStateWithAdd(st.add, ctx1, ctx1')
+          // Additional
+          && st1 == st'
+          && v == MValue(v1, v1')
+        case _ => false
+      })
+  }
+
+  predicate {:verify false} P_Fail(st: S, e: Expr)
+  {
+    var ctx := st.ctx;
+    var ctx' := ctx.(locals := ctx.locals + st.add);
+    var res := InterpExpr(e, st.env, ctx);
+    var res' := InterpExpr(e, st.env, ctx');
+    Inv(st) ==>
+    ExprValid(st, e) ==>
+    res.Failure? && res'.Failure?
+  }
+
+  predicate {:verify false} Pes(st: S, es: seq<Expr>)
+  {
+    var ctx := st.ctx;
+    var ctx' := ctx.(locals := ctx.locals + st.add);
+    var res := InterpExprs(es, st.env, ctx);
+    var res' := InterpExprs(es, st.env, ctx');
+    Inv(st) ==>
+    ExprsValid(st, es) ==>
+    && (match (res, res') {
+        case (Success(Return(vs1, ctx1)), Success(Return(vs1', ctx1'))) =>
+          var st1 := MState(st.env, st.add, ctx1);
+          && EqSeqValue(vs1, vs1')
+          && Inv(st1)
+          && EqStateWithAdd(st.add, ctx1, ctx1')
+        case (Failure(_), _) => true
+        case _ => false
+      })
+  }
+  
+  predicate {:verify false} Pes_Succ(st: S, es: seq<Expr>, st': S, vs: VS)
+  {
+    var ctx := st.ctx;
+    var ctx' := ctx.(locals := ctx.locals + st.add);
+    var res := InterpExprs(es, st.env, ctx);
+    var res' := InterpExprs(es, st.env, ctx');
+    && Inv(st)
+    && ExprsValid(st, es)
+    && (match (res, res') {
+        case (Success(Return(vs1, ctx1)), Success(Return(vs1', ctx1'))) =>
+          var st1 := MState(st.env, st.add, ctx1);
+          && EqSeqValue(vs1, vs1')
+          && Inv(st1)
+          && EqStateWithAdd(st.add, ctx1, ctx1')
+          // Additional
+          && st1 == st'
+          && vs == MSeqValue(vs1, vs1')
+        case _ => false
+      })
+  }
+
+  predicate {:verify false} Pes_Fail(st: S, es: seq<Expr>)
+  {
+    var ctx := st.ctx;
+    var ctx' := ctx.(locals := ctx.locals + st.add);
+    var res := InterpExprs(es, st.env, ctx);
+    var res' := InterpExprs(es, st.env, ctx');
+    Inv(st) ==>
+    ExprsValid(st, es) ==>
+    res.Failure? && res'.Failure?
+  }
+
+
+  function AppendValue ...
+  {
+    MSeqValue([v.v] + vs.vs, [v.v'] + vs.vs')
+  }
+
+  function SeqVToVS ...
+  {
+    if vs == [] then MSeqValue([], [])
+    else
+      AppendValue(MValue(vs[0].v, vs[0].v'), SeqVToVS(vs[1..]))
+  }
+  
+  function GetNilVS ...
+  {
+    MSeqValue([], [])
+  }
+
+  ghost const UnitV := MValue(Values.Unit, Values.Unit)
+
+  function VS_Last ...
+  {
+    var v := vs.vs[|vs.vs| - 1];
+    var v' := vs.vs'[|vs.vs| - 1];
+    MValue(v, v')
+  }
+
+  predicate VS_UpdateStatePre ...
+  {
+    && |argvs.vs| == |argvs.vs'| == |vars|
+    && forall i | 0 <= i < |argvs.vs| :: EqValue(argvs.vs[i], argvs.vs'[i])
+  }
+
+  function {:verify false} BuildClosureCallState ...
+    // Adding this precondition makes the InductAbs proofs easier
+    ensures Inv(st) ==> Inv(st')
+  {
+    var MState(_, add, ctx) := st;
+    var ctx' := ctx.(locals := ctx.locals + add);
+    var ctx1 := BuildCallState(ctx.locals, vars, argvs.vs);
+    var ctx1' := BuildCallState(ctx'.locals, vars, argvs.vs');
+    var st' := MState(env, add, ctx1);
+    assert Inv(st) ==> Inv(st') by {
+      if Inv(st) {
+        assume false; // TODO
+/*        reveal GEqCtx();
+        BuildCallState_EqState(st.ctx.locals, st.ctx'.locals, vars, argvs.vs, argvs.vs');
+        assert EqCtx(ctx1.locals, ctx1'.locals);
+        assert ctx1.rollback == ctx1'.rollback == map [] by {
+          reveal BuildCallState();
+        }*/
+      }
+    }
+    st'
+  }
+
+  function {:verify false} UpdateState ...
+    // Adding this precondition makes the InductUpdate proofs easier
+    ensures Inv(st) ==> Inv(st')
+  {
+    var MState(env, add, ctx) := st;
+    var ctx' := ctx.(locals := ctx.locals + add);
+    var ctx1 := ctx.(locals := AugmentContext(ctx.locals, vars, vals.vs));
+    var ctx1' := ctx'.(locals := AugmentContext(ctx'.locals, vars, vals.vs'));
+    var st' := MState(st.env, st.add, ctx1);
+
+    assert Inv(st) ==> Inv(st') by {
+      if Inv(st) {
+        assume false; // TODO
+/*        reveal BuildCallState();
+        reveal GEqCtx();
+        BuildCallState_EqState(st.ctx.locals, st.ctx'.locals, vars, vals.vs, vals.vs');*/
+      }
+    }
+
+    st'
+  }
+
+  function {:verify false} StateSaveToRollback ...
+    // Rem.(SMH): the proofs in which this is used are ignored (see ``ExprValid``)
+  {
+    var MState(env, add, ctx) := st;
+//    var ctx' := ctx.(locals := ctx.locals + add);
+    var ctx1 := SaveToRollback(ctx, vars);
+    var st' := MState(env, add, ctx1);
+
+    st'
+  }
+
+  function {:verify false} StateBindEndScope ...
+  {
+    var MState(_, _, ctx0) := st0;
+    var MState(env, add, ctx) := st;
+    var ctx1 := ctx.(locals := CtxBindEndScope(ctx0.locals, ctx.locals, vars));
+//    var ctx1' := ctx'.(locals := CtxBindEndScope(ctx0'.locals, ctx'.locals, vars));
+    var st' := MState(env, add, ctx1);
+    st'
+  }
+
+  function {:verify false} StateStartScope ...
+    ensures Inv(st) ==> Inv(st')
+  {
+    var ctx := StartScope(st.ctx);
+//    var ctx' := StartScope(st.ctx');
+//    reveal GEqCtx();
+    var st' := MState(st.env, st.add, ctx);
+    assume Inv(st) ==> Inv(st'); // TODO
+    st'
+  }
+
+  function {:verify false} StateEndScope ...
+//    ensures Inv(st0) && Inv(st) && st.outer_rollback == st.outer_rollback' == EmptyCtx ==> Inv(st')
+  {
+    var ctx := EndScope(st0.ctx, st.ctx);
+//    var ctx' := EndScope(st0.ctx', st.ctx');
+//    reveal GEqCtx();
+    MState(st.env, st.add, ctx)
+  }
+
+  function {:verify false} P_Step ... {
+    var MState(env, add, ctx) := st;
+    var ctx' := ctx.(locals := ctx.locals + add);
+    var Return(v, ctx1) := InterpExpr(e, env, ctx).value;
+    var Return(v', ctx1') := InterpExpr(e, env, ctx').value;
+    (MState(st.env, st.add, ctx1), MValue(v, v'))
+  }
+
+  function {:verify false} Pes_Step ... {
+    var MState(env, add, ctx) := st;
+    var ctx' := ctx.(locals := ctx.locals + add);
+    var Return(vs, ctx1) := InterpExprs(es, env, ctx).value;
+    var Return(vs', ctx1') := InterpExprs(es, env, ctx').value;
+    (MState(st.env, st.add, ctx1), MSeqValue(vs, vs'))
+  }
+
+  //
+  // Lemmas
+  //
+
+  lemma {:verify false} P_Fail_Sound ... {}
+  lemma {:verify false} P_Succ_Sound ... {}
+  lemma {:verify false} Pes_Fail_Sound ... {}
+  lemma {:verify false} Pes_Succ_Sound ... {}
+
+  lemma {:verify false} Pes_Succ_Inj ... {}
+  lemma {:verify false} SeqVToVS_Append ... {}
+
+  lemma {:verify false} InvImpliesEqStateWithAdd(st: S)
+    requires Inv(st)
+    ensures
+      var MState(env, add, ctx) := st;
+      var ctx' := ctx.(locals := ctx.locals + st.add);
+      EqStateWithAdd(add, ctx, ctx')
+  {
+    var MState(env, add, ctx) := st;
+    var ctx' := ctx.(locals := ctx.locals + st.add);
+
+    reveal Inv();
+    assert EqCtx(ctx.locals, ctx'.locals - add.Keys) by {
+      assert ctx'.locals - add.Keys == ctx.locals;
+      reveal GEqCtx();
+      EqCtx_Refl(ctx.locals);
+    }
+    assert add.Keys <= ctx'.locals.Keys;
+    assert forall x | x in add.Keys :: ctx'.locals[x] == add[x];
+    assert ctx.rollback == ctx'.rollback == map [] by { reveal EqStateWithAdd(); }
+    reveal EqStateWithAdd();
+  }
+
+  lemma {:verify false} InductVar ... {
+    reveal InterpExpr();
+    var MState(env, add, ctx) := st;
+    var ctx' := ctx.(locals := ctx.locals + st.add);
+    var v := e.name;
+    
+    // Start by looking in the local context
+    var res0 := TryGetVariable(ctx.locals, v, UnboundVariable(v));
+    var res0' := TryGetVariable(ctx'.locals, v, UnboundVariable(v));
+
+    assert add.Keys !! ctx.locals.Keys by { reveal Inv(); }
+    assert v !in add.Keys by { reveal ExprValid(); }
+
+    InvImpliesEqStateWithAdd(st);
+
+    if res0.Success? {
+      assert res0.Success?;
+      assert v in ctx.locals.Keys;
+      assert v in ctx'.locals.Keys;
+      assert ctx.locals[v] == ctx'.locals[v];
+      EqValue_Refl(ctx.locals[v]);
+    }
+    else {
+      // Not in the local context: look in the global context
+      assert v in env.globals;
+      EqValue_Refl(env.globals[v]);
+    }
+  }
+
+  lemma {:verify false} InductLiteral ... {
+    reveal InterpExpr();
+    reveal InterpLiteral();
+    if Inv(st) {
+      InvImpliesEqStateWithAdd(st);
+    }
+  }
+
+  lemma {:verify true} BuildCallState_EqAdd(st: S, vars: seq<string>, argvs: VS)
+    requires |vars| == |argvs.vs| == |argvs.vs'|
+    requires SeqToSet(vars) !! st.add.Keys
+    ensures
+      var MState(_, add, ctx) := st;
+      var ctx' := ctx.(locals := ctx.locals + st.add);
+      var ctx1 := BuildCallState(ctx.locals, vars, argvs.vs);
+      var ctx1' := BuildCallState(ctx'.locals, vars, argvs.vs');
+      // No, this is false: we use m' instead of m
+      ctx1' == ctx1.(locals := ctx1.locals + add)
+  {
+    var MState(_, add, ctx) := st;
+    var ctx' := ctx.(locals := ctx.locals + st.add);
+//    var ctx1 := BuildCallState(ctx.locals, vars, argvs.vs);
+    var ctx1' := BuildCallState(ctx'.locals, vars, argvs.vs');
+
+//    var m := MapOfPairs(Seq.Zip(vars, argvs.vs));
+    var m' := MapOfPairs(Seq.Zip(vars, argvs.vs'));
+    reveal BuildCallState();
+//    assert ctx1.locals == ctx.locals + m;
+    assert ctx1'.locals == ctx'.locals + m';
+
+    assert st.add.Keys !! m'.Keys by {
+      MapOfPairs_SeqZip_Keys(vars, argvs.vs');
+      reveal SeqToSet();
+    }
+//    assume false;
+//    assert (ctx.locals + st.add) + m' == ctx.locals + (st.add + m');
+    assert (ctx.locals + st.add) + m' == (ctx.locals + m') + st.add;
+    assume false;
+  }
+
+  lemma {:verify true} InductAbs ... {
+    reveal InterpExpr();
+    reveal EqValue_Closure();
+
+    var MState(env, add, ctx) := st;
+    var ctx' := ctx.(locals := ctx.locals + st.add);
+
+    var cv := Values.Closure(ctx.locals, vars, body);
+    var cv' := Values.Closure(ctx'.locals, vars, body);
+
+    forall env, argvs, argvs' |
+      && |argvs| == |argvs'| == |vars|
+      && (forall i | 0 <= i < |vars| :: EqValue(argvs[i], argvs'[i]))
+      ensures
+        var res := InterpCallFunctionBody(cv, env, argvs);
+        var res' := InterpCallFunctionBody(cv', env, argvs');
+        EqPureInterpResultValue(res, res')
+    {
+      // The following triggers instantiations
+      var argvs := MSeqValue(argvs, argvs');
+      assert P(BuildClosureCallState(st, vars, body, env, argvs), body);
+
+      var res := InterpCallFunctionBody(cv, env, argvs.vs);
+      var res' := InterpCallFunctionBody(cv', env, argvs.vs');
+
+      var ctx1 := BuildCallState(cv.ctx, vars, argvs.vs);
+      var ctx1' := BuildCallState(cv'.ctx, cv'.vars, argvs.vs');
+
+//      var m := MapOfPairs(Seq.Zip(vars, argvs.vs));
+//      var m' := MapOfPairs(Seq.Zip(vars, argvs.vs'));
+//      reveal BuildCallState();
+//      assert ctx1.locals == ctx.locals + m;
+//      assert ctx1'.locals == ctx'.locals + m';
+
+      var st1 := BuildClosureCallState(st, vars, body, env, argvs);
+
+//      assert 
+      assert ctx1' == ctx1.(locals := ctx1.locals + add) by { // TODO: this is false. Update the invariant
+        assert SeqToSet(vars) !! st.add.Keys by {
+          reveal SeqToSet();
+          reveal ExprValid();
+        }
+        BuildCallState_EqAdd(st, vars, argvs);
+      }
+      assert Inv(st1);
+      assert st1 == MState(env, add, ctx1);
+      assert P(st1, body);
+      
+      var res2 := InterpExpr(cv.body, env, ctx1);
+      var res2' := InterpExpr(cv'.body, env, ctx1');
+
+      reveal InterpCallFunctionBody();
+
+      assert Inv(st1);
+      assume ExprValid(st1, body); // TODO
+
+      if res2.Success? {
+        var Return(val, ctx2) := res2.value;
+        var Return(val', ctx2') := res2'.value;
+      }
+      else {
+        assert res.Failure?;
+      }
+    }
+
+    InvImpliesEqStateWithAdd(st);
+    assert EqValue_Closure(cv, cv');
+  }
+
+  lemma {:verify false} InductAbs_CallState ... {
+    reveal InterpExpr();
+    reveal InterpCallFunctionBody();
+    reveal BuildCallState();
+  }
+
+  lemma {:verify false} InductExprs_Nil ... {
+    assume false; // TODO
+    reveal InterpExprs(); }
+  lemma {:verify false} InductExprs_Cons ... {
+    assume false; // TODO
+    reveal InterpExprs(); }
+
+  lemma {:verify false} InductApplyLazy_Fail ... {
+    assume false; // TODO
+    reveal InterpExpr(); }
+  lemma {:verify false} InductApplyLazy_Succ ... {
+    assume false; // TODO
+    reveal InterpExpr(); }
+
+  lemma {:verify false} InductApplyEager_Fail ... {
+    assume false; // TODO
+  }
+
+  lemma {:verify false} InductApplyEagerUnaryOp_Succ ... {
+    assume false; // TODO
+  }
+
+  lemma {:verify false} InductApplyEagerBinaryOp_Succ ... {
+    assume false; // TODO
+    reveal InterpExpr();
+//    InterpBinaryOp_Eq(e, e, op, v0.v, v1.v, v0.v', v1.v');
+  }
+
+  lemma {:verify false} {:fuel SeqVToVS, 2} InductApplyEagerTernaryOp_Succ ... {
+    assume false; // TODO
+    reveal InterpExpr();
+    // TODO(SMH): ``SeqVToVS`` is called on literals: we shouldn't need fuel 2
+//    assert SeqVToVS([v0, v1, v2]) == MSeqValue([v0.v, v1.v, v2.v], [v0.v', v1.v', v2.v']);
+//    InterpTernaryOp_Eq(e, e, op, v0.v, v1.v, v2.v, v0.v', v1.v', v2.v');
+  }
+
+  lemma {:verify false} InductApplyEagerBuiltinDisplay ... {
+    assume false; // TODO
+    reveal InterpExpr();
+//    Interp_Apply_Display_EqValue(e, e, ty.kind, argvs.vs, argvs.vs');
+  }
+
+  lemma {:verify false} InductApplyEagerFunctionCall ... {
+    assume false; // TODO
+    reveal InterpExpr();
+//    InterpFunctionCall_EqState(e, e, st.env, fv.v, fv.v', argvs.vs, argvs.vs');
+  }
+
+  lemma {:verify false} InductIf_Fail ... {
+    assume false; // TODO
+    reveal InterpExpr(); }
+  lemma {:verify false} InductIf_Succ ... {
+    assume false; // TODO
+    reveal InterpExpr(); }
+
+  lemma {:verify false} InductUpdate_Fail ... {
+    assume false; // TODO
+    reveal InterpExpr(); }
+  lemma {:verify false} InductUpdate_Succ ... {
+    assume false; // TODO
+    reveal InterpExpr(); }
+
+  lemma {:verify false} InductVarDecl_None_Succ ... {
+    assume false; // TODO
+    reveal InterpExpr(); }
+  lemma {:verify false} InductVarDecl_Some_Fail ... {
+    assume false; // TODO
+    reveal InterpExpr(); }
+  lemma {:verify false} InductVarDecl_Some_Succ  ... {
+    assume false; // TODO
+    reveal InterpExpr(); }
+
+  lemma {:verify false} InductBind_Fail ... {
+    assume false; // TODO
+    reveal InterpExpr(); }
+  lemma {:verify false} InductBind_Succ ... {
+    assume false; // TODO
+    reveal InterpExpr();
+
+    // Sanity check: there are issues in ``EqInterpScopes``
+/*    var MState(env, _, ctx, _, ctx') := st;
+    assert InterpExpr(e, env, ctx) == Success(Return(v.v, st4.ctx));
+    assert InterpExpr(e, env, ctx') == Success(Return(v.v', st4.ctx'));
+
+    reveal GEqCtx();*/
+  }
+
+  // TODO(SMH): I tried simplifying the proofs below by adding a `requires` in ``InductBlock_Fail``
+  // and ``InductBlock_Succ`` to provide the result of calling ``InterpExprs_Block_Equiv_Strong``,
+  // but it didn't work due to SMT solvers' misteries.
+  lemma {:verify false} InductBlock_Fail ...
+  {
+    assume false; // TODO
+    reveal InterpExpr();
+    reveal InterpBlock();
+    reveal InterpExprs();
+    reveal InterpBlock_Exprs();
+    reveal InterpExprs_Block();
+    
+//    InterpExprs_Block_Equiv_Strong(stmts, st.env, st_start.ctx);
+//    InterpExprs_Block_Equiv_Strong(stmts, st.env, st_start.ctx');
+  }
+
+  lemma {:verify false} InductBlock_Succ ...
+  {
+    assume false; // TODO
+    reveal InterpExpr();
+    reveal InterpBlock();
+    reveal InterpExprs();
+    reveal InterpBlock_Exprs();
+    reveal InterpExprs_Block();
+    
+//    InterpExprs_Block_Equiv_Strong(stmts, st.env, st_start.ctx);
+//    InterpExprs_Block_Equiv_Strong(stmts, st.env, st_start.ctx');
+  }
 }
+
